theories/L/Computability/Por.v
@@ -1,5 +1,5 @@
 From Undecidability.L.Functions Require Export Eval.
-From Undecidability.L.Tactics Require Import Lbeta_nonrefl.
+
 (* * Definition of parallel or *)
 
 Section hoas. Import HOAS_Notations.
@@ -22,7 +22,7 @@ Proof.
   -Lproc.
   -eexists;now Lsimpl.
   -Lsimpl. edestruct (doesHaltIn s n) eqn:eq;unfold doesHaltIn in eq;rewrite H in eq. 2:congruence. reflexivity.
-  -eapply Seval.eval_converges. unfold Por. Lsimpl_old. rewrite R. Lsimpl. Lreflexivity.
+  -eapply Seval.eval_converges. unfold Por. Lsimpl. rewrite R. Lsimpl. Lreflexivity.
 Qed.
 
 Lemma Por_correct_1b (s t:term) : converges t -> converges (Por (ext s) (ext t)).
@@ -32,7 +32,7 @@ Proof.
   -Lproc.
   -eexists;now Lsimpl.
   -Lsimpl.  edestruct (doesHaltIn t n) eqn:eq;unfold doesHaltIn in eq;rewrite H in eq. 2:congruence. edestruct doesHaltIn;reflexivity.
-  -eapply Seval.eval_converges. unfold Por. Lsimpl_old. rewrite R. Lsimpl. Lreflexivity.
+  -eapply Seval.eval_converges. unfold Por. Lsimpl. rewrite R. Lsimpl. Lreflexivity.
 Qed.
 
 Lemma Por_correct_1 s t : converges s \/ converges t -> converges (Por (ext s) (ext t)).
@@ -48,7 +48,7 @@ Proof.
   apply app_converges in C as [_ [v' [C lv']]].
   assert (C':=C).
   apply mu_sound in C as [n [eq [R' H]]];try Lproc.
-  -exists (doesHaltIn s n). subst. unfold Por. Lsimpl_old. rewrite C'. now Lsimpl. 
+  -exists (doesHaltIn s n). subst. unfold Por. Lsimpl. rewrite C'. now Lsimpl. 
   -eexists. now Lsimpl.
 Qed.
 
