theories/L/Datatypes/LUnit.v
@@ -5,6 +5,3 @@ From Undecidability.L.Tactics Require Import LTactics GenEncode.
 
 MetaCoq Run (tmGenEncodeInj "unit_enc" unit).
 #[export] Hint Resolve unit_enc_correct : Lrewrite.
-
-Lemma size_unit_enc : size(enc tt) = 2. 
-Proof. reflexivity. Qed. 
