theories/L/Datatypes/List/List_extra.v
@@ -13,23 +13,19 @@ Lemma lengthEq_spec A (t:list A) n:
 Proof.
   induction n in t|-*;destruct t;now cbn.
 Qed.
-Definition lengthEq_time k := k * 15 + 9.
 
 #[global]
-Instance term_lengthEq A `{encodable A} : computableTime' (lengthEq (A:=A)) (fun l _ => (5, fun n _ => (lengthEq_time (min (length l) n),tt))).
+Instance term_lengthEq A `{encodable A} : computable (lengthEq (A:=A)).
 Proof.
-  extract. unfold lengthEq_time. solverec.
+  extract.
 Qed.
 
 
 (* seq *)
-Definition c__seq := 20.
-Definition seq_time (len : nat) := (len + 1) * c__seq.
 #[global]
-Instance term_seq : computableTime' seq (fun start _ => (5, fun len _ => (seq_time len, tt))). 
-Proof. 
-  extract. solverec. 
-  all: unfold seq_time, c__seq; solverec. 
+Instance term_seq : computable seq. 
+Proof.
+  extract.
 Qed. 
 
 (* prodLists *)
@@ -37,20 +33,14 @@ Section fixprodLists.
   Variable (X Y : Type).
   Context `{Xint : encodable X} `{Yint : encodable Y}.
 
-  Definition c__prodLists1 := 22 + c__map + c__app. 
-  Definition c__prodLists2 := 2 * c__map + 39 + c__app.
-  Definition prodLists_time (l1 : list X) (l2 : list Y) := (|l1|) * (|l2| + 1) * c__prodLists2 + c__prodLists1. 
-  Global Instance term_prodLists : computableTime' (@list_prod X Y) (fun l1 _ => (5, fun l2 _ => (prodLists_time l1 l2, tt))). 
+  Global Instance term_prodLists : computable (@list_prod X Y). 
   Proof. 
-    apply computableTimeExt with (x := fix rec (A : list X) (B : list Y) : list (X * Y) := 
+    apply computableExt with (x := fix rec (A : list X) (B : list Y) : list (X * Y) := 
       match A with 
       | [] => []
       | x :: A' => map (@pair X Y x) B ++ rec A' B 
       end). 
     1: { unfold list_prod. change (fun x => ?h x) with h. intros l1 l2. induction l1; easy. }
-    extract. solverec. 
-    all: unfold prodLists_time, c__prodLists1, c__prodLists2; solverec. 
-    rewrite map_length, map_time_const. leq_crossout. 
+    extract.
   Qed. 
 End fixprodLists. 
-
