theories/L/Tactics/Reflection.v
@@ -1,6 +1,6 @@
 From Undecidability.L Require Export Util.L_facts.
-From Undecidability.L.Tactics Require Export LClos_Eval.
-From Undecidability.L.Tactics Require Import mixedTactics.
+From Undecidability.L.Tactics Require Import LClos.
+Require Import ZArith. (* ? *)
 Require Import FunInd.
 
 (* *** Reflexted closure calculus *)
